pancake/semantics/crepSemScript.sml
@@ -245,7 +245,7 @@ Definition evaluate_def:
        (case (read_bytearray w2 (w2n w) (mem_load_byte s.memory s.memaddrs s.be),
               read_bytearray w4 (w2n w3) (mem_load_byte s.memory s.memaddrs s.be)) of
          | SOME bytes,SOME bytes2 =>
-            (case call_FFI s.ffi ffi_index bytes bytes2 of
+            (case call_FFI s.ffi (explode ffi_index) bytes bytes2 of
               | FFI_final outcome => (SOME (FinalFFI outcome),s)
               | FFI_return new_ffi new_bytes =>
                 (case write_bytearray w4 new_bytes s.memory s.memaddrs s.be of
